---
marp: true
---
<style>
  section {
    font-family: 'LXGW Bright';
  }

  h1, h2, h3 {
    font-family: 'LXGW Bright';
  }
</style>
<style>
img[alt~="center"] {
  display: block;
  margin: 0 auto;
}
</style>
<style>
.note {
  background-color: #eef;
  padding: 10px;
  margin: 10px 0;
  text-align: left;
}
.trick {
  background-color: #fee;
  padding: 10px;
  margin: 10px 0;
  text-align: left;
}
</style>

# Series

Speaker: Yixiao Qian

---

## Table of Contents

<br>

- Numerical Series
- Function Sequences and Series
- Power Series

---

# Numerical Series

---

## Concept of Numerical Series

<br>

- **Convergence**: $S_n = \sum_{k=1}^n u_k$ is parital-sum, $S_n$ converges.
- **Necessary Condition**: $\lim \limits _{n \rightarrow \infty} u_n = 0$. (Since $\lim \limits _{n \rightarrow \infty} u_n = \lim \limits _{n \rightarrow \infty} S_n - \lim \limits _{n \rightarrow \infty} S_{n-1} = 0$)
- **Cauchy Criterion**: $\forall \epsilon > 0, \exists N > 0, N < m < m+p$, $|u_{m+1} + \cdots + u_{m+p}| < \epsilon$.

---

## Positive-Term Series

- **Integral Test**: $f$ non-negative and decreasing, then $\displaystyle \sum_{n=1}^{\infty} f(n) \sim \int_1^{+\infty}f(x) \mathrm{d} x$.

<div class=note>

$\sum_{n=1}^{\infty} \frac{1}{n^p}$ converges when $p > 1$, diverges when $p \leq 1$.

</div>

- **Comparison Test**: If $u_n \sim v_n$ when $n \rightarrow \infty$, then $\sum_{n=1}^{\infty} u_n \sim \sum_{n=1}^{\infty}v_n$.
- **Ratio Test**: $\lim \limits _{n \rightarrow \infty} \frac{u_{n+1}}{u_n} = q$. $q<1$ then $\sum u_n$ converges, $q > 1$ then diverges.
- **Root Test**: $\lim \limits _{n \rightarrow \infty} \sqrt[n]{u_n} = q$. $q <ï¼‘$ then $\sum u_n$ converges, $q > 1$ then diverges.

---

## Arbitrary-Term Series

---

# Function Sequences and Series

---

## Uniform Convergence of Function Sequence

- **Uniform Convergence**: $\forall \epsilon > 0$, $\exists N > 0$, $\forall n > N$, $|f_n(x) - f(x)| < \epsilon$ holds for all $x \in D$.
- **Cauchy Criterion**: $\forall \epsilon > 0$, $\exists N > 0$, $\forall m,m+p > N$, $|f_{m+p}(x)-f_{m}(x)| < \epsilon$ holds for $x \in D$
- **Compact Convergence**: $f_n \rightrightarrows f$ on any closed/compact subset of $D$.

<div class=note>

Motivation: Continuous functions on closed sets are uniformly continuous.

</div>

- **Weiestrass Test**: If $|f(x) - f_n(x)| \leq a_n$ for all $x$, $\lim \limits _{n \rightarrow \infty} a_n = 0$ is positive-term, then $f_n \rightrightarrows f$
- **Closure under Operations**: $kf_n$, $f_n+g_n$, $f_ng_n$ (if bounded), $1/f_n$ (if no roots).
- **Uniform Boundedness**: $\exists M > 0$, $\forall n > 0$, $|f_n(x)| \leq M$ for all $x$.
- **Boundedness of Limit Function**: If $f_n \rightarrow f$ pointwisely. Then $f_n \rightrightarrows f$, $f_n$ bounded > $f_n$ uniformly bounded > $f$ bounded.

---

## Practice on Concept of Uniform Convergence

- If $f$ has continuous derivative on $(0, 1)$, $f_n(x) = n[f(x+\frac{1}{n}) - f(x)]$. Prove that $f_n(x)$ is uniformly convergent on any closed subset of $(0, 1)$.

<div class=note>

</div>

---

## Properties of Limit Function: Continuity

- **Local Continuity**: $f_n \rightrightarrows f$ on $(a, b)$, $\lim \limits _{x \rightarrow x_0}f_n(x) = a_n$, then $\lim \limits _{x \rightarrow x_0}f(x) = \lim \limits _{n \rightarrow \infty} a_n$. 

<div class=note>

Note: The result can also be written as $\lim \limits _{n \rightarrow \infty} \lim \limits _{x \rightarrow x_0} f_n(x) = \lim \limits _{x \rightarrow x_0} \lim \limits _{n \rightarrow \infty} f_n(x)$.
(1) Existence of $\lim \limits _{n \rightarrow \infty} a_n$: By $f_n \rightrightarrows f$, then $\forall \epsilon > 0$, $\exists N > 0$, $\forall m,n > N$, $|f_n(x) - f_m(x)| < \epsilon$. Take $x \rightarrow x_0$, then $|a_n - a_m| < \epsilon$, which means $A = \lim \limits _{n \rightarrow \infty} a_n$ exists (Cauchy's criterion).
(2) $\lim \limits _{x \rightarrow x_0}f(x) = A$: $|f(x) - A| \leq |f(x) - f_n(x)| + |f_n(x) - a_n| + |a_n - A| < 3\epsilon$.

</div>

- **Global Continuity**: $f_n$ are continuous on $(a, b)$, $f_n \rightrightarrows f$ on any closed subset, then $f$ is continuous. ($f_n \rightrightarrows f$ on the entire $(a, b)$ is stronger)

</div>

- **Uniform Continuity**: $f_n$ uniformly continuous, $f_n \rightrightarrows f$, then $f$ is uniformly continuous.

<div class=note>

Consider $|f(x_1) - f(x_2)| \leq |f(x_1) - f_n(x_1)| + |f_n(x_1) - f_n(x_2)| + |f_n(x_2) - f(x_2)| < 3 \epsilon$.

</div>

---

## Properties of Limit Function: Integrability

---

## Properties of Limit Function: Differentiability


---

# Power Series

---

## Convergence Behavior of Power Series

- **Abel's Theorem**: (1) $\sum a_nx_0^n$ converges, for $|x| < |x_0|$, $\sum a_nx^n$ converges absolutely. (2) $\sum a_nx_0^n$ diverges, for $|x| > |x_0|$, $\sum a_nx^n$ diverges.
- **Radius of Convergence**: $|x| < R$, $\sum a_nx^n$ converges absolutely; $|x| > R$, $\sum a_nx^n$ diverges.
- **Cauchy-Hadamard Test**: $\frac{1}{R} = \lim \limits _{n \rightarrow \infty} \sqrt[n]{|a_n|}$.
- **Ratio Test**: $\frac{1}{R} = \lim \limits _{n \rightarrow \infty} \frac{|a_{n+1}|}{|a_n|}$.
- Find the Convergence Region: (1) $\sin x$ and $\cos x$, (2) $e^x$, (3) $\ln (1+x)$, (4) $\frac{1}{1-x}$.

<div class=note>

(1) $\sin x = \sum_{n=0}^{\infty} (-1)^n \frac{x^{2n+1}}{(2n+1)!}$, $\frac{1}{R} = \sqrt[n]{\frac{1}{(2n+1)!}} \rightarrow 0$, then $R = \infty$. So is $\cos x$.
(2) $e^x = \sum_{n=0}^{\infty} \frac{x^n}{n!}$, $\frac{1}{R} = \sqrt[n]{\frac{1}{n!}} \rightarrow 0$. Then $R = \infty$.
(3) $\ln x = \sum_{n=1}^{\infty} (-1)^{n-1} \frac{x^n}{n}$, $\frac{1}{R} = \sqrt[n]{\frac{1}{n}} \rightarrow 1$. Then $R = 1$. The convergence region is $(-1,1]$.
(4) $\frac{1}{1-x} = \sum_{n=0}^{\infty} x^n$, $\frac{1}{R} = \sqrt[n]{1} = 1$. The convergence region is $(-1,1)$.

</div>

---

## Sum Function of Power Series




---

## Power Series Expansion

- **Expansion of Rational Functions**: $f(x) = \frac{x^2}{x^2 - 3x + 1}$

<div class=note>

(1) Decompose: $\frac{x^2}{x^2-3x+1} = 1 + \frac{4}{x-2} - \frac{1}{x-1}$ (Method of Undetermined Coefficients)
(2) $\frac{1}{x-2} = -\frac{1}{2} \cdot \frac{1}{1 - \frac{x}{2}} = - \frac{1}{2} \sum\limits_{n=0}^{\infty} \left( \frac{x}{2} \right)^n$ and $\frac{1}{x-1} = - \frac{1}{1-x} = - \sum\limits_{n = 0}^{\infty} x^n$.

</div>

- **Take Integration**: $f(x) = \frac{1}{(1+x)^2}$.

<div class=note>

Consider $\displaystyle F(x) = \int_0^x \frac{1}{(1+t)^2}\mathrm{d} t$. Then $F(x) = -\frac{1}{1+x} + 1 = 1 - \sum_{n=0}^{\infty} (-x)^n$. $f(x) = F^{\prime}(x)$.

</div>

- **Take Derivative**: (1) $f(x) = \arctan x$, (2) $f(x) = \arctan \frac{1-kx}{1+kx}$.

<div class=note>

(1) $f^{\prime}(x) = \frac{1}{1+x^2} = \sum_{n=0}^{\infty}(-1)^nx^{2n}$. Then $f = \sum_{n=0}^{\infty} (-1)^n \frac{x^{2n+1}}{2n+1}$.

</div>



